floyd/efield_lemmas.v
@@ -1,45 +1,13 @@
 Require Import floyd.base.
 Require Import floyd.assert_lemmas.
 Require Import floyd.client_lemmas.
-Require Import floyd.fieldlist.
+Require Import floyd.nested_pred_lemmas.
 Require Import floyd.nested_field_lemmas.
 Local Open Scope logic.
 
 Inductive LLRR : Type :=
   | LLLL : LLRR
   | RRRR : LLRR.
-
-Definition type_almost_match e t lr:=
-  match typeof e, t, lr with
-  | Tpointer t0 a0, Tarray t1 _ a1, RRRR => eqb_type (typeof e) (Tpointer t1 a1)
-  | _, _, LLLL => eqb_type (typeof e) t
-  | _, _, _ => false
-  end.
-
-Fixpoint legal_nested_efield_rec t_root e (gfs: list gfield) (tts: list type) lr: bool :=
-  match gfs, tts with
-  | nil, nil => type_almost_match e t_root lr
-  | nil, _ => false
-  | _ , nil => false
-  | gf :: gfs0, t0 :: tts0 => 
-    match nested_field_rec t_root gfs with
-    | Some (_, ttt) => (legal_nested_efield_rec t_root e gfs0 tts0 lr && eqb_type ttt t0)%bool
-    | None => false
-    end
-  end.
-
-Definition legal_nested_efield env t_root e gfs tts lr :=
-  match gfs, tts, lr with
-  | nil, nil, RRRR => false
-  | nil, nil, LLLL => eqb_type (uncompomize env t_root) (typeof e)
-  | nil, _, _ => false
-  | _ , nil, _ => false
-  | gf :: gfs0, t0 :: tts0, _ => 
-    match nested_field_rec t_root gfs with
-    | Some (_, ttt) => (legal_nested_efield_rec t_root e gfs0 tts0 lr && eqb_type (uncompomize env ttt) t0)%bool
-    | None => false
-    end
-  end.
 
 Inductive efield : Type :=
   | eArraySubsc: forall i: expr, efield
@@ -62,8 +30,8 @@ Fixpoint compute_nested_efield e : expr * list efield * list type :=
   match e with
   | Efield e' id t => 
     match compute_nested_efield e', typeof e' with
-    | (e'', efs, tts), Tstruct _ _ _ => (e'', eStructField id :: efs, t :: tts)
-    | (e'', efs, tts), Tunion _ _ _ => (e'', eUnionField id :: efs, t :: tts)
+    | (e'', efs, tts), Tstruct _ _ => (e'', eStructField id :: efs, t :: tts)
+    | (e'', efs, tts), Tunion _ _ => (e'', eUnionField id :: efs, t :: tts)
     | _, _ => (e, nil, nil)
     end
   | Ederef (Ebinop Oadd e' ei (Tpointer t a)) t' =>
@@ -81,17 +49,17 @@ Definition compute_lr e (efs: list efield) :=
   | _, _ => LLLL
   end.
 
-Fixpoint efield_denote (efs: list efield) (gfs: list gfield) : environ -> mpred :=
+Fixpoint efield_denote (Delta: tycontext) (efs: list efield) (gfs: list gfield) : environ -> mpred :=
   match efs, gfs with
   | nil, nil => TT
   | eArraySubsc ei :: efs', ArraySubsc i :: gfs' => 
-    local (`(eq (Vint (Int.repr i))) (eval_expr ei)) &&
+    local (`(eq (Vint (Int.repr i))) (eval_expr Delta ei)) &&
     !! (match typeof ei with | Tint _ _ _ => True | _ => False end) &&
-    efield_denote efs' gfs'
+    efield_denote Delta efs' gfs'
   | eStructField i :: efs', StructField i0 :: gfs' =>
-    !! (i = i0) && efield_denote efs' gfs'
+    !! (i = i0) && efield_denote Delta efs' gfs'
   | eUnionField i :: efs', UnionField i0 :: gfs' =>
-    !! (i = i0) && efield_denote efs' gfs'
+    !! (i = i0) && efield_denote Delta efs' gfs'
   | _, _ => FF
   end.
 
@@ -106,21 +74,6 @@ Fixpoint tc_efield (Delta: tycontext) (efs: list efield) rho : Prop :=
     tc_efield Delta efs' rho
   end.
 
-(*
-Lemma legal_nested_efield_cons: forall env t_root gf gfs t tts ,
-  legal_nested_efield env t_root (gf :: gfs) (t :: tts) = true ->
-  legal_nested_efield env t_root gfs tts = true.
-Proof.
-Opaque nested_field_rec.
-  intros.
-  simpl in H.
-  valid_nested_field_rec t_root (gf :: gfs) H.
-  solve_nested_field_rec_cons_eq_Some H0;
-  rewrite andb_true_iff in H;
-  tauto.
-Transparent nested_field_rec.
-Qed.
-*)
 Lemma compute_nested_efield_aux: forall e t,
   match compute_nested_efield e with
   | (e', gfs, tts) => nested_efield e' gfs tts = e
@@ -169,6 +122,57 @@ Proof.
   auto.
 Qed.
 
+Section CENV.
+
+Context {cs: compspecs}.
+
+Definition type_almost_match e t lr:=
+  match typeof e, t, lr with
+  | Tpointer t0 a0, Tarray t1 _ a1, RRRR => eqb_type (typeof e) (Tpointer t1 a1)
+  | _, _, LLLL => eqb_type (typeof e) t
+  | _, _, _ => false
+  end.
+
+Fixpoint legal_nested_efield_rec t_root e (gfs: list gfield) (tts: list type) lr: bool :=
+  match gfs, tts with
+  | nil, nil => type_almost_match e t_root lr
+  | nil, _ => false
+  | _ , nil => false
+  | gf :: gfs0, t0 :: tts0 => 
+    match nested_field_rec t_root gfs with
+    | Some (_, ttt) => (legal_nested_efield_rec t_root e gfs0 tts0 lr && eqb_type ttt t0)%bool
+    | None => false
+    end
+  end.
+
+Definition legal_nested_efield t_root e gfs tts lr :=
+  match gfs, tts, lr with
+  | nil, nil, RRRR => false
+  | nil, nil, LLLL => eqb_type t_root (typeof e)
+  | nil, _, _ => false
+  | _ , nil, _ => false
+  | gf :: gfs0, t0 :: tts0, _ => 
+    match nested_field_rec t_root gfs with
+    | Some (_, ttt) => (legal_nested_efield_rec t_root e gfs0 tts0 lr && eqb_type ttt t0)%bool
+    | None => false
+    end
+  end.
+
+(*
+Lemma legal_nested_efield_cons: forall env t_root gf gfs t tts ,
+  legal_nested_efield env t_root (gf :: gfs) (t :: tts) = true ->
+  legal_nested_efield env t_root gfs tts = true.
+Proof.
+Opaque nested_field_rec.
+  intros.
+  simpl in H.
+  valid_nested_field_rec t_root (gf :: gfs) H.
+  solve_nested_field_rec_cons_eq_Some H0;
+  rewrite andb_true_iff in H;
+  tauto.
+Transparent nested_field_rec.
+Qed.
+*)
 (*
 Lemma legal_nested_efield_nested_field_rec_isSome: forall env t_root e gfs tts lr,
   legal_nested_efield env t_root e gfs tts lr = true -> isSome (nested_field_rec t_root gfs).
@@ -184,10 +188,10 @@ Transparent nested_field_rec.
 Qed.
 *)
 
-Lemma typeof_nested_efield: forall env Delta t_root e efs gfs tts lr,
-  legal_nested_efield env t_root e gfs tts lr = true ->
-  local (tc_efield Delta efs) && efield_denote efs gfs |--
-    !! (uncompomize env (nested_field_type2 t_root gfs) = typeof (nested_efield e efs tts)).
+Lemma typeof_nested_efield: forall Delta t_root e efs gfs tts lr,
+  legal_nested_efield t_root e gfs tts lr = true ->
+  local (tc_efield Delta efs) && efield_denote Delta efs gfs |--
+    !! (nested_field_type2 t_root gfs = typeof (nested_efield e efs tts)).
 Proof.
 Admitted.
 (*
@@ -218,20 +222,20 @@ Transparent nested_field_rec.
 Qed.
 *)
 
-Lemma offset_val_sem_add_pi: forall ofs t0 e rho i,
+Lemma offset_val_sem_add_pi: forall Delta ofs t0 e rho i,
    offset_val (Int.repr ofs)
-     (force_val (sem_add_pi t0 (eval_expr e rho) (Vint (Int.repr i)))) =
+     (force_val (sem_add_pi Delta t0 (eval_expr Delta e rho) (Vint (Int.repr i)))) =
    offset_val (Int.repr ofs)
-     (offset_val (Int.mul (Int.repr (sizeof t0)) (Int.repr i)) (eval_expr e rho)).
+     (offset_val (Int.mul (Int.repr (sizeof (composite_types Delta) t0)) (Int.repr i)) (eval_expr Delta e rho)).
 Proof.
   intros.
-  destruct (eval_expr e rho); try reflexivity.
+  destruct (eval_expr Delta e rho); try reflexivity.
 Qed.
 
 Lemma By_reference_eval_expr: forall Delta e rho,
   access_mode (typeof (e)) = By_reference ->
   tc_lvalue Delta e rho ->
-  eval_expr e rho = eval_lvalue e rho.
+  eval_expr Delta e rho = eval_lvalue Delta e rho.
 Proof.
   intros.
   unfold tc_lvalue in H0.
@@ -393,10 +397,10 @@ Proof.
   Admitted.
 *)
 
-Definition eval_LR e lr :=
+Definition eval_LR Delta e lr :=
   match lr with
-  | LLLL => eval_lvalue e
-  | RRRR => eval_expr e
+  | LLLL => eval_lvalue Delta e
+  | RRRR => eval_expr Delta e
   end.
 
 Definition tc_LR Delta e lr :=
@@ -405,14 +409,14 @@ Definition tc_LR Delta e lr :=
   | RRRR => tc_expr Delta e
   end.
 
-Lemma eval_lvalue_nested_efield_aux: forall Delta env t_root e efs gfs tts lr,
-  legal_nested_efield env t_root e gfs tts lr = true ->
-  local (`isptr (eval_LR e lr)) && local (tc_LR Delta e lr) &&
-    local (tc_efield Delta efs) && efield_denote efs gfs |--
-  local (`isptr (eval_lvalue (nested_efield e efs tts))) &&
+Lemma eval_lvalue_nested_efield_aux: forall Delta t_root e efs gfs tts lr,
+  legal_nested_efield t_root e gfs tts lr = true ->
+  local (`isptr (eval_LR Delta e lr)) && local (tc_LR Delta e lr) &&
+    local (tc_efield Delta efs) && efield_denote Delta efs gfs |--
+  local (`isptr (eval_lvalue Delta (nested_efield e efs tts))) &&
     local (tc_lvalue Delta (nested_efield e efs tts)) &&
-    local (`eq (eval_lvalue (nested_efield e efs tts))
-      (`(field_address t_root gfs) (eval_LR e lr))).
+    local (`eq (eval_lvalue Delta (nested_efield e efs tts))
+      (`(field_address t_root gfs) (eval_LR Delta e lr))).
 Proof.
 Admitted.
 (*
@@ -539,22 +543,22 @@ Opaque classify_add.
 Qed.
 *)
 
-Lemma eval_lvalue_nested_efield: forall Delta env t_root e efs gfs tts lr,
-  legal_nested_efield env t_root e gfs tts lr = true ->
-  local (`isptr (eval_LR e lr)) && local (tc_LR Delta e lr) &&
-  local (tc_efield Delta efs) && efield_denote efs gfs |-- local (`eq (eval_lvalue (nested_efield e efs tts))
-      (`(field_address t_root gfs) (eval_LR e lr))).
+Lemma eval_lvalue_nested_efield: forall Delta t_root e efs gfs tts lr,
+  legal_nested_efield t_root e gfs tts lr = true ->
+  local (`isptr (eval_LR Delta e lr)) && local (tc_LR Delta e lr) &&
+  local (tc_efield Delta efs) && efield_denote Delta efs gfs |-- local (`eq (eval_lvalue Delta (nested_efield e efs tts))
+      (`(field_address t_root gfs) (eval_LR Delta e lr))).
 Proof.
   intros.
   eapply derives_trans; [eapply eval_lvalue_nested_efield_aux; eauto |].
   simpl; intros; normalize.
 Qed.
 
-Lemma tc_lvalue_nested_efield: forall Delta env t_root e efs gfs tts lr,
-  legal_nested_efield env t_root e gfs tts lr = true ->
-  local (`isptr (eval_LR e lr)) && local (tc_LR Delta e lr) &&
-  local (tc_efield Delta efs) && efield_denote efs gfs |--
-    local (`isptr (eval_lvalue (nested_efield e efs tts))) &&
+Lemma tc_lvalue_nested_efield: forall Delta t_root e efs gfs tts lr,
+  legal_nested_efield t_root e gfs tts lr = true ->
+  local (`isptr (eval_LR Delta e lr)) && local (tc_LR Delta e lr) &&
+  local (tc_efield Delta efs) && efield_denote Delta efs gfs |--
+    local (`isptr (eval_lvalue Delta (nested_efield e efs tts))) &&
     local (tc_lvalue Delta (nested_efield e efs tts)).
 Proof.
   intros.
@@ -562,3 +566,4 @@ Proof.
   simpl; intros; normalize.
 Qed.
 
+End CENV.
